Implement test about a specific register (RDRAND)

experimental/drng/Test.Hacl.Hardware.Intel.CPUID.fst
@@ -1,52 +1,47 @@
 module Test.Hacl.Hardware.Intel.CPUID
 
+open FStar.ST
+open FStar.HyperStack
+open FStar.Buffer
+open FStar.UInt32
+
 open Hacl.Hardware.Intel.CPUID
 
 
 
-(* (\* Default value of a cpuid_t structure *\) *)
-(* let id:cpuid_t = { *)
-(*   eax = 0ul; *)
-(*   ebx = 0ul; *)
-(*   ecx = 0ul; *)
-(*   edx = 0ul; *)
-(* } *)
-
-
 (* Detect if the processor is an Intel CPU *)
-val detect_intel_cpu: unit -> St bool
+val detect_intel_cpu: unit 
+  -> Stack bool
+          (requires (fun h -> True))
+          (ensures  (fun h0 _ h1 -> h0 == h1))
 let detect_intel_cpu () = if (_is_intel_cpu() = 1ul) then true else false
 
 
 (* Detect if the processor has support for the DRNG features *)
-val detect_intel_feature_rdrand: unit -> St bool
+val detect_intel_feature_rdrand: unit
+  -> Stack bool (requires (fun h0 -> True))
+               (ensures  (fun h0 _ h1 -> modifies_0 h0 h1))
+               
 let detect_intel_feature_rdrand () =
-  match detect_intel_cpu () with
-  | false -> false
-  | true -> true
-
-
-(* Int intel_check_drng(){ *)
-
-(*   // Check if the processor is an Intel CPU *)
-(*   if ( _is_intel_cpu()) { *)
-(*     cpuid_t features; *)
-
-(*     // Get the CPU information *)
-(*     // Check for the RDRAND feature bit *)
-(*     cpuid(&features, 1, 0); *)
-
-(*     if (features.ecx & 0x40000000 == 0x40000000) { *)
-(*       return 0; *)
-(*     } *)
-(*   } *)
-(*   return 1; *)
-(* } *)
-
-
-let main () =
   push_frame();
+  let features = { eax = 0ul; ebx = 0ul; ecx = 0ul; edx = 0ul; } in
+  let rfeatures = Buffer.create features 1ul in
+  let r =
+    match detect_intel_cpu () with
+    | false -> false
+    | true ->
+      (* Retrieve the cpuid information from the CPU *)
+      cpuid rfeatures 1ul 0ul;
+      (* Check the bit for the RDRAND feature *)
+      if ((let a = rfeatures.(0ul) in a.ecx &^ 0x40000000ul) =^ 0x40000000ul) then true else false
+  in
+  pop_frame();
+  r
 
+
+(* Entry point *)
+let main () =
+  
   (* Detect if the machine is an Intel CPU *)
   (match detect_intel_cpu () with
   | true  -> C.print_string (C.string_of_literal " * CPU Information: Intel processor detected on your machine.\n")
@@ -57,5 +52,4 @@ let main () =
   | true -> C.print_string (C.string_of_literal " *         Feature: Digital Random Number Generator (RDRAND)\n")
   | false -> ());
 
-  pop_frame();
   C.exit_success
